hop2: prf

proof/correctness/Hop2.ec
@@ -7,25 +7,36 @@ from Jasmin require import JModel JArray.
 require import Params Parameters Address Notation Primitives Wots Generic.
 require import RandomBytes XMSS_IMPL XMSS_IMPL_HOP1.
 
-require import Array2 Array3 Array8 Array32 Array67 Array2144.
+require import Array2 Array3 Array8 Array32 Array64 Array67 Array96 Array128 Array2144.
 
-require import Utils. (* valid ptr predicate & addr_to_bytes *)
+require import Utils. (* valid ptr predicate & W64ToBytes & addr_to_bytes *)
 require import Correctness_Mem. (* memcpy results *)
 (*---*) import NBytes.
 require import Termination.
 
+require import BitEncoding.
+(*---*) import BitChunking.
+
 
 op padding_len : int.
-op prf_padding_val : W8.t.
-op prf_kg_padding_val : W8.t.
+op padding_val : W64.t.
 
 module Hop2 = {
+  proc w64_to_bytes (x : W64.t, outlen : int) = {
+    var r : W8.t list;
+    
+    (* TODO: FIX THIS *)
+    r <- nseq outlen W8.zero;
+  
+    return r;
+  } 
+
   proc prf (in_0 : W8.t list, key : nbytes) : nbytes = {
     var r : nbytes;
     var padding : W8.t list;
     var buf : W8.t list;
 
-    padding <- nseq padding_len prf_padding_val;
+    padding <@ w64_to_bytes (padding_val, padding_len);
     buf <- padding ++ key ++ in_0;
 
     r <- Hash buf;
@@ -38,7 +49,7 @@ module Hop2 = {
     var padding : W8.t list;
     var buf : W8.t list;
 
-    padding <- nseq padding_len prf_kg_padding_val;
+    padding <@ w64_to_bytes (padding_val, padding_len);
     buf <- padding ++ key ++ in_0;
 
     r <- Hash buf;
@@ -56,7 +67,7 @@ module Hop2 = {
     var i : int;
     var t : W8.t;
     
-    padding <- nseq padding_len prf_padding_val;
+    padding <@ w64_to_bytes (padding_val, padding_len);
     addr_bytes <- addr_to_bytes address;
     u <@ prf (addr_bytes, seed);
 
@@ -105,30 +116,193 @@ module Hop2 = {
     
     return (t, address);
    }
+
+   proc pseudorandom_genSK(sk_seed : nbytes, seed : nbytes, address : adrs) : wots_sk * adrs= {
+       var sk : wots_sk <- nseq len (nseq n witness);
+       var sk_i : nbytes;
+       var i : int;
+       var addr_bytes : W8.t list;
+    
+       address <- set_hash_addr address 0;
+       address <- set_key_and_mask address 0;
+
+       i <- 0;
+       while (i < len) {
+       address <- set_chain_addr address i;
+       addr_bytes <- addr_to_bytes address;
+       sk_i <@ prf_keygen ((seed ++ addr_bytes), sk_seed);
+       sk <- put sk i sk_i;
+       i <- i + 1;
+     }
+
+         return (sk, address);
+  }
+
 }.
 
+(*** ***)
 
-lemma prf_hop2 (a b : W8.t Array32.t) :
-    equiv [
-    M(Syscall).__prf ~ Hop2.prf : 
-    arg{1}.`2 = a /\ arg{1}.`2 = b /\ arg{2} = (to_list a, to_list b) 
-    ==>
-    res{2} = to_list res{1}
-    ].
+lemma ull_to_bytes_correct (x : W64.t) : 
+    equiv [M(Syscall).__ull_to_bytes_32 ~ Hop2.w64_to_bytes :
+      arg{1}.`2 = x /\ arg{2} = (x, 32)  ==> res{2} = to_list res{1}].
 proof.
 proc.
 admit.
 qed.
 
 
+axiom hash_96 (x : W8.t Array96.t) :
+    phoare[M(Syscall).__core_hash_96 : arg.`2 = x ==> to_list res = Hash (to_list x)] = 1%r.
+
+axiom hash_128 (x : W8.t Array128.t) :
+    phoare[M(Syscall).__core_hash_128 : arg.`2 = x ==> to_list res = Hash (to_list x)] = 1%r.
+
+
 lemma prf_hop2 (a b : W8.t Array32.t) :
+    padding_val = XMSS_HASH_PADDING_PRF /\ padding_len = XMSS_PADDING_LEN =>
     equiv [
     M(Syscall).__prf ~ Hop2.prf : 
+    arg{1}.`2 = a /\ arg{1}.`3 = b /\ arg{2} = (to_list a, to_list b) 
+    ==>
+    res{2} = to_list res{1}
+    ].
+proof.
+rewrite /XMSS_HASH_PADDING_PRF /XMSS_PADDING_LEN ; move => [p_val p_len].
+proc.
+seq 9 2 : (buf{2} = to_list buf{1}); last first.
+  + inline M(Syscall).__core_hash__96 M(Syscall)._core_hash_96; wp; sp.
+    ecall {1} (hash_96 buf{1}); auto => /> /#.
+seq 3 0 : (#pre); 1:auto.
+seq 1 1 : (#pre /\ padding{2} = to_list padding_buf{1}).
+  + call {1} (ull_to_bytes_correct (of_int 3)%W64); auto => />. 
+seq 1 0 : (
+  key{2} = to_list key{1} /\
+  in_0{2} = to_list in_0{1} /\
+  padding{2} = to_list padding_buf{1} /\ 
+  forall (k : int), 0 <= k < 32 => buf{1}.[k] = nth witness padding{2} k
+); first by auto => /> *; smt(@Array96 @List).
+seq 1 0 : (#pre /\ aux{1} = key{1}); first by ecall {1} (_x_memcpy_u8u8_post key{1}); auto => />.
+seq 1 0 : (#pre /\ forall (k : int), 32 <= k < 64 => buf{1}.[k] = nth witness key{2} (k - 32)).
+    + auto => />; smt(@Array96 @List).
+seq 1 0 : (
+  key{2} = to_list key{1} /\
+  in_0{2} = to_list in_0{1} /\
+  padding{2} = to_list padding_buf{1} /\ 
+  (forall (k : int), 0 <= k < 32 => buf{1}.[k] = nth witness padding{2} k) /\
+  (forall (k : int), 32 <= k < 64 => buf{1}.[k] = nth witness key{2} (k - 32)) /\
+  aux{1} = in_0{1}
+).
+    + ecall {1} (_x_memcpy_u8u8_post in_0{1}); auto => /> /#.
+seq 1 0 : (
+  key{2} = to_list key{1} /\ size key{2} = 32 /\
+  in_0{2} = to_list in_0{1} /\ size in_0{2} = 32 /\
+  padding{2} = to_list padding_buf{1} /\  size padding{2} = 32 /\
+  (forall (k : int), 0 <= k < 32 => buf{1}.[k] = nth witness padding{2} k) /\
+  (forall (k : int), 32 <= k < 64 => buf{1}.[k] = nth witness key{2} (k - 32)) /\
+  (forall (k : int), 64 <= k < 96 => buf{1}.[k] = nth witness in_0{2} (k - 64))
+).
+    + auto => /> *; do split; smt(@Array96 @List).
+    + auto => /> *; rewrite !/to_list !/mkseq -!iotaredE => /> /#. 
+qed.
+
+
+lemma prf_keygen_hop2 (a b : W8.t Array64.t) :
+    equiv [
+    M(Syscall).__prf_keygen ~ Hop2.prf : 
     arg{1}.`2 = a /\ arg{1}.`2 = b /\ arg{2} = (to_list a, to_list b) 
     ==>
     res{2} = to_list res{1}
     ].
 proof.
 proc.
+seq 9 2 : (buf{2} = to_list buf{1}); last first.
+  + inline M(Syscall).__core_hash__128 M(Syscall)._core_hash_128; wp; sp.
+    ecall {1} (hash_128 buf{1}); auto => /> /#.
+admit.
+qed.
+
+(*** ***)
+
+op encode_wots_sk (sk_spec : wots_sk) : W8.t Array2144.t =
+    Array2144.of_list witness (flatten sk_spec).
+
+lemma expand_seed_correct (
+    _in_seed : W8.t Array32.t, _pub_seed : W8.t Array32.t, _addr : W32.t Array8.t):
+    len = XMSS_WOTS_LEN /\ n = XMSS_N =>
+    equiv [M(Syscall).__expand_seed ~ Hop2.pseudorandom_genSK :
+      arg{1}.`2 = _in_seed /\ 
+      arg{1}.`3 = _pub_seed /\
+      arg{1}.`4 = _addr /\
+      arg{2} = (to_list _in_seed, to_list _pub_seed, _addr) ==>
+      res{1}.`1 = encode_wots_sk res{2}.`1 /\ 
+      res{1}.`2 = res{2}.`2].
+proof.
+rewrite /XMSS_WOTS_LEN /XMSS_N; move => [len_val n_val].
+proc; auto => />.
+conseq (: _ ==>  addr{1} = address{2} /\ forall (k : int), 0 <= k < 2144 => outseeds{1}.[k] = nth witness (flatten sk{2}) k).
+  + auto => /> rL rR. rewrite /encode_wots_sk. rewrite /of_list. auto => />. admit.
+seq 3 1 : (
+  #pre /\
+  buf{1} = witness /\
+  ith_seed{1} = witness /\
+  addr_bytes{1} = witness /\
+  size sk{2} = len /\
+  size (flatten sk{2}) = 2144
+).
+    + auto => />. split; smt(@List).
+seq 2 2 : ( (* Same as # pre but without addr{1/2} = _addr *)
+  inseed{1} = _in_seed /\
+  pub_seed{1} = _pub_seed /\
+  sk_seed{2} = to_list _in_seed /\
+  seed{2} = to_list _pub_seed /\
+  ith_seed{1} = witness /\ 
+  size sk{2} = len /\ 
+  size (flatten sk{2}) = 2144 /\
+  addr{1} = address{2}
+); first by inline {1}; auto => />.
+seq 1 0 : (#pre /\ aux{1} = pub_seed{1}); first by ecall {1} (_x_memcpy_u8u8_post pub_seed{1}); auto => />.
+seq 1 0 : (#pre /\ (forall (k : int), 0 <= k < 32 => buf{1}.[k] = pub_seed{1}.[k])); first by auto => /> *; smt(@Array64).
+while (
+  (* This is from pre *)
+  size sk{2} = len /\ size (flatten sk{2}) = 2144 /\
+  
+  0 <= i{1} <= 67 /\ ={i} /\
+
+  addr{1} = address{2} /\
+  addr_bytes{2} = to_list addr_bytes{1} /\
+  sk_i{2} = to_list ith_seed{1} /\
+  buf{1} = Array64.of_list witness (seed{2} ++ addr_bytes{2}) /\
+  
+  forall (k : int), 0 <= k < 32 * i{2} => outseeds{1}.[k] = nth witness (flatten sk{2}) k
+); last first.
++ auto => /> &1 &2 *. do split.
+    - admit.
+    - admit.
+    - admit.
+    - smt(@List @Array2144).
+    - by rewrite len_val.
+    - move => *. admit.
+seq 1 1 : (#pre); first by inline {1}; auto => />.
+auto => />.
+    + move => &1 &2. move => [#] ?????????????????. move => [#] ?????????????. do split.
+        * smt().
+        * smt().
+        * smt().
+        * smt().
+        * smt().
+        * smt().
+        * smt().
+        * smt().
+        * smt().
+        * auto => /> k *. rewrite initE. case (0 <= k && k < 2144); last by smt(). move => ?. 
+          case (i{1} * 32 <= k && k < i{1} * 32 + 32); 1,2:by move => ?; smt(@List @Array2144). 
+        * smt().
+        * smt().
+auto => />.
+(*
+seq 1 0 : (#pre). auto => /> &1 &2 *. apply (eq_from_nth witness). by rewrite !size_to_list. admit.
+seq 1 1 : (#pre).
+    + ecall {1} (addr_to_bytes_correctness addr{1}). auto => /> &1 &2 *. admit.
+*)
 admit.
 qed.
